Fixed initial phases up-to L3->L4 proof

theories/L1g/term.v
@@ -1209,7 +1209,7 @@ Inductive WFTrm: Term -> nat -> Prop :=
 with WFTrmBs: Brs -> nat -> Prop :=
      | wfbnil: forall n, WFTrmBs bnil n
      | wfbcons: forall n m b bs,
-         WFTrm b n -> WFTrmBs bs n -> WFTrmBs (bcons m b bs) n
+         WFTrm b (List.length m + n) -> WFTrmBs bs n -> WFTrmBs (bcons m b bs) n
 with WFTrmDs: Defs -> nat -> Prop :=
      | wfdnil: forall n, WFTrmDs dnil n
      | wfdcons: forall n nm bod arg ds,
@@ -1577,6 +1577,11 @@ Qed.
 End Instantiate_sec.
 End PoccTrm_sec.
 
+Fixpoint instantiatel s k t :=
+  match s with
+  | [] => t
+  | a :: s => instantiatel s k (instantiate a (List.length s + k) t)
+  end.
 
 Lemma instantiate_pres_WFapp:
   (forall bod, WFapp bod ->
@@ -1670,7 +1675,10 @@ unfold whBetaStep; simpl; induction 1; intros.
 
 Definition whCaseStep (cstrNbr:nat) (args:Terms) (brs:Brs): option Term := 
   match bnth cstrNbr brs with
-    | Some (t, _) => Some (mkApp t args)
+    | Some (t, argnames) =>
+      if eqb (List.length argnames) (List.length args) then 
+        Some (instantiatel args 0 t)
+      else None
     | None => None
   end.
 
@@ -1700,7 +1708,7 @@ Qed.
 
 Lemma bnth_pres_WFTrm:
   forall n (brs:Brs), WFTrmBs brs n ->
-    forall m x ix, bnth m brs = Some (x, ix) -> WFTrm x n.
+    forall m x ix, bnth m brs = Some (x, ix) -> WFTrm x (List.length ix + n).
 Proof.
   intros n brs h m x ix.
   functional induction (bnth m brs); intros; auto.
@@ -1709,6 +1717,14 @@ Proof.
   - apply IHo; inversion h; assumption.
 Qed.
 
+Lemma instantiates_pres_WFapp bod s k : 
+  WFapp bod -> WFapps s -> 
+  WFapp (instantiatel s k bod).
+Proof.
+  induction s in bod |- *; cbn; auto.
+  intros h h'; inv h'.
+  eapply IHs; auto. now eapply instantiate_pres_WFapp.
+Qed.
 
 Lemma whCaseStep_pres_WFapp:
   forall (brs:Brs), WFappBs brs -> forall ts, WFapps ts -> 
@@ -1716,9 +1732,11 @@ Lemma whCaseStep_pres_WFapp:
 Proof.
   intros brs hbrs ts hts n s h. unfold whCaseStep in h.
   case_eq (bnth n brs); intros; rewrite H in h.
-  - destruct p. myInjection h. apply mkApp_pres_WFapp.
-    + assumption.
-    + eapply (bnth_pres_WFapp hbrs n). eassumption.
+  - destruct p. 
+    destruct (eqb_spec (List.length l) (List.length ts)); try discriminate.
+    myInjection h.
+    eapply (bnth_pres_WFapp hbrs n) in H.
+    now eapply instantiates_pres_WFapp.
   - discriminate.
 Qed.
 
