theories/L4_deBruijn/toplevel.v
@@ -2,9 +2,6 @@ Require Import L4.expression.
 Require Import Common.Common Common.compM Common.Pipeline_utils.
 Require Import L2k.compile.
 Require Import L4.L3_to_L4.
-Require Import L4.L3_to_L3_eta.
-Require Import L4.L3_eta_crct.
-Require Import L4.L3_to_L3_eta_correct.
 Require Import L4.L3_to_L4_correct.
 Require L2k.
 Require Import BinNat.
@@ -13,28 +10,16 @@ Import Monads.
 
 Import MonadNotation.
 
-
-Definition L3_eta_Program := Program L2k.compile.Term.
-Typeclasses Opaque L3_eta_Program.
-
-Definition compile_L2k_eta
-  : CertiCoqTrans (Program L2k.compile.Term) L3_eta_Program:=
-  fun src =>
-    debug_msg "Translating from L2k to L2k - eta expansion" ;;
-    (LiftCertiCoqTrans "L2k_eta" L3_to_L3_eta.Program_Program src).
-
-(* TODO instance for correctness proof *)
-
 Definition L4Term := prod ienv L4.expression.exp.
 
-Instance L4_Lang : Lang L4Term :=
+#[global] Instance L4_Lang : Lang L4Term :=
   { Value := L4.expression.exp ;
     TermWf := fun P => L4.expression.exp_wf (0%N) (snd P);
     BigStep := fun P Res => exists n, L4.expression.eval_n n (snd P) = Some Res
   }.
 
 Definition compile_L4 (prims : list (kername * string * nat * positive))
-  : CertiCoqTrans L3_eta_Program L4Term :=
+  : CertiCoqTrans (Program L2k.compile.Term) L4Term :=
   fun src =>
     debug_msg "Translating from L2k to L4" ;;
     LiftCertiCoqTrans "L4" (fun p =>  
